3162. b)
$$
\begin{align}
\frac{\sqrt[3]{y^2}}{\sqrt[3]{y}*\sqrt[3]{y^4}}=\sqrt[3]{\frac{y^2}{y*y^4}}=\sqrt[3]{\frac{y^2}{y^5}}=\sqrt[3]{\frac{1}{y^3}} = \frac{1}{y}
\end{align}
$$
3162. c)
$$
\frac{\sqrt[4]{a}*\sqrt[4]{a^5}}{\sqrt[4]{a^3}*\sqrt[4]{a^2}*\sqrt[4]{a^{-3}}}=\sqrt[4]{\frac{a*a^5}{a^3*a^2*a^{-3}}}=\sqrt[4]{\frac{a^6}{a^2}}=\sqrt[4]{a^4}=a
$$
3162. e)
$$
\frac{\sqrt[3]{a^{-2}}*\sqrt[4]{a^3}}{\sqrt{a^{-3}}*\sqrt[6]{a^{-5}}}=\frac{\sqrt[12]{a^{-8}}*\sqrt[12]{a^9}}{\sqrt[12]{a^{-18}}*\sqrt[12]{a^{-10}}}=\sqrt[12]{\frac{a^{-8}*a^9}{a^{-18}*a^{-10}}}=\sqrt[12]{\frac{a}{a^{-28}}}=\sqrt[12]{a^{29}}
$$
3162. d)
$$
\frac{\sqrt[3]{a^2*b^{-1}}*\sqrt[3]{a^{-2}*b^{-4}}}{\sqrt[3]{a^5*b^{-3}}*\sqrt[3]{a^{-2}*b^{-1}}}=\sqrt[3]{\frac{a^2*b^{-1}*a^{-2}*b^4}{a^5*b^{-3}*a^{-4}*b^{-1}}}=\sqrt[3]{\frac{b^3}{a*b^{-4}}}=\sqrt[3]{\frac{b^7}{a}}
$$
3162. f)
$$
\frac{\sqrt[4]{a^{-1}*b^3}*\sqrt[6]{a^5*b^{-3}}}{\sqrt[3]{a^4*b^2}*\sqrt{a^3*b^-3}}=\sqrt[12]{\frac{a^{-3}*b^9*a^{10}*b^{-6}}{a^{16}*b^{-8}*a^{16}*b^{18}}}=\sqrt[12]{\frac{a^7*b^3}{a^{34}*b^{-26}}} =\sqrt[12]{\frac{b^{29}}{a^{27}}}
$$
# HW
3162. g)
3163. a, b, c)